steel/README.md
@@ -1,3 +1,1 @@
-You need the steel branch of F* to compile code in this directory
-AF (Jun 5, 2021), recent changes to the Steel VC generation seem to have broken normalization of VCs, verification currently fails.
-For now, use the steel_icfp21 branch.
+You need the master branch of F* to compile code in this directory
